packages/pickles-circuit-diffs/src/Pickles/CircuitDiffs/PureScript/StepMainChunks2.purs
@@ -101,6 +101,7 @@ compileStepMainChunks2 params = do
           { perSlotLagrangeAt: Vector.nil
           , blindingH: params.blindingH
           , perSlotFopDomainLog2s: Vector.nil
+          , perSlotFopZkRows: Vector.nil
           , perSlotVkBlueprints: unit
           }
           dummyWrapSg
