packages/pickles-circuit-diffs/src/Pickles/CircuitDiffs/PureScript/StepMainNoRecursionReturn.purs
@@ -100,6 +100,7 @@ compileStepMainNoRecursionReturn params = do
           { perSlotLagrangeAt: Vector.nil
           , blindingH: params.blindingH
           , perSlotFopDomainLog2s: Vector.nil
+          , perSlotFopZkRows: Vector.nil
           , perSlotVkBlueprints: unit
           }
           dummyWrapSg
